stuff

Caches/StoreAtomicity.v
@@ -2,8 +2,8 @@ Require Import DataTypes Transitions Useful.
 
 Set Implicit Arguments.
 
-Inductive InstantMemory : (Addr -> Data) -> (Addr -> Data) -> Set :=
-| IReq m a (p: Proc) d (w: Desc):
+Inductive InstantMemory m : (Addr -> Data) -> Set :=
+| IReq a (p: Proc) d (w: Desc):
   InstantMemory m (if w
                    then m
                    else 
@@ -11,14 +11,14 @@ Inductive InstantMemory : (Addr -> Data) -> (Addr -> Data) -> Set :=
                        if decAddr a a'
                        then d
                        else m a')
-| IIdle m: InstantMemory m m.
+| IIdle: InstantMemory m m.
 
 Definition getImIo s s' (t: InstantMemory s s') :=
   match t with
-    | IReq m a p d w => Some (a, p, d, w, if w
-                                          then m a
+    | IReq a p d w => Some (a, p, d, w, if w
+                                          then s a
                                           else initData zero)
-    | IIdle m => None
+    | IIdle => None
   end.
 
 Section CreateInstantMemory.
@@ -28,7 +28,6 @@ Section CreateInstantMemory.
   Variable stm: Stream Trans initState.
   Variable getTransIo: forall s s',
                          Trans s s' -> option (Addr * Proc * Data * Desc * Data). 
-
   Record StoreAtomicity := {
    storeAtomicityLd:
     forall t a c d ld,
@@ -49,43 +48,75 @@ Section CreateInstantMemory.
      getStreamIo getTransIo t stm = Some (a, c, d, St, ld) ->
      ld = initData zero }.
 
-  CoFixpoint buildIm n m: Stream InstantMemory m :=
-  TCons _ (match getStreamIo getTransIo n stm as use
-              return (InstantMemory m match use with
-                                        | Some (a, _, d, w, _) => if w
-                                                                  then m
-                                                                  else fun a' =>
-                                                                         if decAddr a a'
-                                                                         then d
-                                                                         else m a'
-                                        | None => m
-                                      end) with
-             | Some (a, c, d, w, ld) => (IReq m a c d w)
-             | None => (IIdle m)
-           end) (buildIm (S n) (match getStreamIo getTransIo n stm as use
-                                   return (Addr -> Data) with
-                                  | Some (a, c, d, w, ld) => if w
-                                                             then m
-                                                             else fun a' =>
-                                                                    if decAddr a a'
-                                                                    then d
-                                                                    else m a'
-                                  | None => m
-                                end)).
+  Fixpoint getNStateForStm x :=
+    match x with
+      | 0 => initData
+      | S m => match getStreamIo getTransIo m stm with
+                 | Some (a, c, d, w, ld) => if w
+                                            then getNStateForStm m
+                                            else fun a' =>
+                                                   if decAddr a a'
+                                                   then d
+                                                   else (getNStateForStm m) a'
+                 | None => getNStateForStm m
+               end
+    end.
+
+  CoFixpoint buildIm n: Stream InstantMemory (getNStateForStm n) :=
+    TCons _
+          (match getStreamIo getTransIo n stm as io return InstantMemory (getNStateForStm n)
+              match io with
+                | Some (a, c, d, w, ld) => if w
+                                           then getNStateForStm n
+                                           else fun a' => if decAddr a a'
+                                                          then d
+                                                          else (getNStateForStm n) a'
+                | None => getNStateForStm n
+              end
+             with
+               | Some (a, c, d, w, ld) => IReq (getNStateForStm n) a c d w
+               | None => IIdle (getNStateForStm n)
+             end) (eq_rect_r _ (buildIm (S n)) eq_refl).
+
+
+  Theorem buildImSth n:
+    forall m,
+      match getStreamIo getTransIo (n+m) stm, getStreamIo getImIo n (buildIm m) with
+        | Some (a, c, d, w, ld), Some (a', c', d', w', ld') =>
+          a = a' /\ c = c' /\ d = d' /\ w = w' /\
+          ld' = if w then getNStateForStm (n+m) a else initData zero
+        | None, None => True
+        | _, _ => False
+      end.
+  Proof.
+    unfold getStreamIo, getImIo.
+    induction n.
+    intros.
+    simpl in *.
+    unfold getStreamIo.
+    destruct (getTransIo (getStreamTransition stm m)).
+    destruct p,p,p,p; intuition.
+    intuition.
+    intros.
+    specialize (IHn (S m)).
+    assert (n + S m = S n + m) by omega.
+    rewrite H in *.
+    assumption.
+  Qed.
 End CreateInstantMemory.
 
 Section AllSa.
-
-  Theorem memGood t:
+  Theorem memGood' t:
     forall s (stm: Stream InstantMemory s) a,
-    (forall ti,
+    (fst (getStreamState t stm) a = s a /\
+     forall ti,
        0 <= ti < t ->
        forall ci di ldi,
          ~ getStreamIo getImIo ti stm = Some (a, ci, di, St, ldi)) \/
     (exists cb tb ldb,
        tb < t /\
        getStreamIo getImIo tb stm =
-       Some (a, cb, fst (getStreamState tb stm) a, St, ldb) /\
+       Some (a, cb, fst (getStreamState t stm) a, St, ldb) /\
        forall ti, tb < ti < t ->
                   forall ci di ldi,
                     ~ getStreamIo getImIo ti stm = Some (a, ci, di, St, ldi)).
@@ -95,7 +126,7 @@ Section AllSa.
     intros.
     simpl in *.
     destruct stm; simpl.
-    constructor; (reflexivity || intuition; assert False by omega; intuition).
+    left; (reflexivity || intuition; assert False by omega; intuition).
 
     intros.
 
@@ -105,9 +136,13 @@ Section AllSa.
     destruct i; intros; simpl in *.
     destruct w.
 
-    destruct (IHt _ stm a) as [nopast|past].
+    destruct (IHt _ stm a) as [[cond nopast]|past].
 
-    left; intros; destruct ti; simpl in *.
+    left; intros.
+    constructor.
+    assumption.
+    intros;
+      destruct ti; simpl in *.
     discriminate.
     assert (0 <= ti < t) by omega;
       apply (nopast); intuition.
@@ -126,151 +161,349 @@ Section AllSa.
     assert (tb < ti < t) by omega.
     apply (rest (ti) H2 ci di ldi H).
 
-    specialize (IHt _ stm a).
 
-    destruct (decAddr a0 a).
+    destruct (decAddr a0 a); intros.
     rewrite <- e in *.
 
-    right; intros.
+    right.
+    destruct (IHt _ stm a) as [[cond nopast]|past]; clear IHt.
+
     exists p, 0, (initData zero).
+
     constructor.
     omega.
     simpl.
+    constructor.
+    destruct (decAddr a0 a).
+    destruct (decAddr a0 a0); intuition.
 
-as [nopast|past].
-
-    
-    intros.
-
+    rewrite <- e in *.
+    rewrite cond in *.
     intuition.
-    pose proof (nextStmEq ti stm).
-    simpl in H.
-    simpl in *.
-    unfold getStreamIo in *; intuition.
+    intuition.
     intros.
-    destruct ti;
-      unfold getStreamIo in *; simpl in *;
-             [discriminate | assert (tb < ti < t) by omega].
-    apply (rest ti H0 ci di ldi).
+
+    destruct ti.
+    omega.
+    simpl in *.
+    rewrite <- e in *.
+    assert (H2: 0 <= ti < t) by omega.
+    apply (nopast _ H2 ci di ldi).
+
+    match goal with
+      | H: exists cb tb ld, _ |- _ =>
+          destruct H as [cb [tb [ldb [eq1 [eq2 rest]]]]];
+          exists cb, (S tb), ld
+    end.
+    constructor; (omega || intuition).
+
+    rewrite <- e in *.
+    intuition.
+
+    destruct ti.
+    omega.
+    simpl in *.
+    assert (tb < ti < t) by omega.
+    rewrite <- e in *.
+    apply (rest (ti) H2 ci di ldi H).
+
+    destruct (decAddr a0 a).
+    intuition.
+
+    destruct (IHt _ stm a) as [[cond nopast] | past]; clear IHt.
+    
+    destruct (decAddr a0 a).
+    intuition.
+
+    left; intros.
+    constructor.
+    assumption.
+    intros;
+      destruct ti; simpl in *.
+    unfold not; intros. injection H0; intros.
+    intuition.
+    assert (0 <= ti < t) by omega;
+      apply (nopast); intuition.
+
+    right; intros.
+    match goal with
+      | H: exists cb tb ld, _ |- _ =>
+          destruct H as [cb [tb [ldb [eq1 [eq2 rest]]]]];
+          exists cb, (S tb), ld
+    end.
+    constructor; (omega || intuition).
+
+    destruct ti.
+    omega.
+    simpl in H.
+    assert (tb < ti < t) by omega.
+    apply (rest (ti) H2 ci di ldi H).
 
     specialize (IHt _ stm a).
+    destruct IHt as [[cond nopast] | past].
 
-    destruct (decAddr a0 a).
-    rewrite e in *.
-                               match goal with
-                                 | nopast: _ /\ _ |- _ =>
-                                     destruct nopast as [_ nopast];
-                                     apply nopast; intuition
-                               end].
-    assert (S tb < S t
-    simpl.
-
-    
-
-    destruct tb;
-      unfold getStreamIo in *; simpl in *.
-    destruct stm; simpl in *.
-             [discriminate | intuition].
-    unfold getStreamIo in *; discriminate.
-
-    unfold getStreamIo in *; simpl.
-    assert (0 <= ti < t) by omega.
-    destruct H as [_ u2].
-
-    apply (u2 _ H1 ci di ldi).
-    simpl in *; discriminate.
-    simpl in *.
-    destruct opts.
-    rewrite H0.
-    simpl.
-    intros; discriminate.
-    simpl.
-    simpl.
-    assert (0 <= 
-    specialize (u2
-    unfold getStreamTransition.
-    simpl.
-    About getStreamTransition.
-    simpl.
-    
-    
-    intros.
-
-    specialize (IHt a).
-    destruct IHt.
+    left; intros.
     constructor.
-    constructor.
-    specialize (IHt a); intuition.
-    
+    assumption.
+    intros; destruct ti; simpl in *.
+    discriminate.
 
-    specialize (IHt a).
-    destruct (decAddr a0 a).
-    rewrite e in *.
+    assert (0 <= ti < t) by omega;
+      apply nopast; intuition.
 
-    simpl in *.
+    right; intros.
 
-        getStreamIo getImIo t stm = Some (a, c, d, Ld, ld) -> Some (a, ci, di, St, ldi)
-      (ld = mem a /\
-     forall {ti}, 0 <= ti < t -> forall ci di ldi, defined ci ->
-                                   ~ getStreamIo getImIo ti stm = Some (a, ci, di, St, ldi)) \/
-    (exists cb tb ldb, defined cb /\ tb < t /\ getStreamIo getImIo tb stm = Some (a, cb, ld, St, ldb) /\
-      forall ti, tb < ti < t ->
-                   forall ci di ldi, defined ci ->
-                     ~ getStreamIo getImIo ti stm = Some (a, ci, di, St, ldi)).
-  Proof.
+    match goal with
+      | H: exists cb tb ld, _ |- _ =>
+          destruct H as [cb [tb [ldb [eq1 [eq2 rest]]]]];
+          exists cb, (S tb), ld
+    end.
+    constructor; (omega || intuition).
 
+    destruct ti.
+    omega.
 
-  Theorem storeAtomicityLd' t:
-    forall mem (stm: Stream InstantMemory mem) a c d ld,
+    simpl in H.
+    assert (tb < ti < t) by omega.
+    apply (rest (ti) H2 ci di ldi H).
+  Qed.
+
+  Theorem storeAtomicityLd':
+    forall mem (stm: Stream InstantMemory mem) t a c d ld,
       getStreamIo getImIo t stm = Some (a, c, d, Ld, ld) ->
       (ld = mem a /\
-     forall {ti}, 0 <= ti < t -> forall ci di ldi, defined ci ->
+     forall {ti}, 0 <= ti < t -> forall ci di ldi, 
                                    ~ getStreamIo getImIo ti stm = Some (a, ci, di, St, ldi)) \/
-    (exists cb tb ldb, defined cb /\ tb < t /\ getStreamIo getImIo tb stm = Some (a, cb, ld, St, ldb) /\
+    (exists cb tb ldb, tb < t /\ getStreamIo getImIo tb stm = Some (a, cb, ld, St, ldb) /\
       forall ti, tb < ti < t ->
-                   forall ci di ldi, defined ci ->
+                   forall ci di ldi, 
                      ~ getStreamIo getImIo ti stm = Some (a, ci, di, St, ldi)).
   Proof.
-    induction t.
+    pose proof memGood'.
     intros.
-
+    specialize (H t mem stm a).
     unfold getStreamIo, getImIo in *.
-    simpl in *.
-    destruct stm.
-    destruct i.
-    destruct w.
-    injection H; intros.
-    rewrite H3, H2, H1, H0 in *.
+    destruct (getStreamTransition stm t).
+    injection H0. intros.
+
+    rewrite H2, H3, H4, H5, H1 in *.
+    destruct H.
     left.
-    constructor; intuition.
-    discriminate.
-    discriminate.
+    intuition.
+    right.
 
+    destruct H as [cb [tb [ldb rest]]].
+    exists cb, tb, ldb.
+    intuition.
+    discriminate.
+  Qed.
+
+  Theorem storeAtomicitySt':
+    forall s (stm: Stream InstantMemory s) t a c d ld,
+      getStreamIo getImIo t stm = Some (a, c, d, St, ld) ->
+      ld = initData zero.
+  Proof.
     intros.
-    unfold getStreamIo, getImIo in *.
+    unfold getImIo, getStreamIo in *.
+    destruct (getStreamTransition stm t).
+    destruct w.
+    discriminate.
+    injection H; auto.
+    discriminate.
+  Qed.
+
+  Definition saInstMem (stm: Stream InstantMemory initData) 
+                        := Build_StoreAtomicity
+                             stm getImIo (storeAtomicityLd' stm) (storeAtomicitySt' stm).
+End AllSa.
+
+Section Final.
+  Variable State: Set.
+  Variable Trans: AllTransitions State.
+  Variable initState: State.
+  Variable stm: Stream Trans initState.
+  Variable (getTransIo: forall s s', Trans s s' -> option (Addr * Proc * Data * Desc * Data)).
+  Variable sa: StoreAtomicity stm getTransIo.
+
+  Theorem buildImSimulate:
+    forall n,
+    getStreamIo getTransIo n stm = getStreamIo getImIo n (buildIm stm getTransIo 0).
+  Proof.
+    apply (@ind (fun n => getStreamIo getTransIo n stm = getStreamIo getImIo n
+                                                                     (buildIm stm getTransIo 0))).
+    simpl in *.
+    destruct sa as [sLd sSt].
+
+    pose proof (saInstMem (buildIm stm getTransIo 0)) as [bLd bSt].
+    specialize (sLd 0).
+    specialize (sSt 0).
+    specialize (bLd 0).
+    specialize (bSt 0).
+
+    pose proof (buildImSth stm getTransIo 0 0) as sth; assert (H:0+0 = 0) by omega;
+    rewrite H in *; clear H.
+
     simpl in *.
 
-    destruct stm.
-    specialize (IHt s' stm a c d ld H).
-    unfold getStream
-    injection H; intros.
-    assert (sth: fst (getStreamState 0 stm) = initData).
-    simpl.
-    destruct stm.
-    reflexivity.
-    destruct stm.
-    unfold getImIo in *.
-    destruct i.
-    destruct w.
-    injection H; intros.
-    rewrite H3, H2, H1, H0 in *.
-    simpl.
-    simpl.
-    destruct stm.
-    unfold getStreamS
-    assert (fst (match stm with
-                   | TCons s0 s' _ _ => (s0, s'
-    destruct stm.
-    simpl.
-End AllSa.
-*)
+    destruct (getStreamIo getTransIo 0 stm).
+    destruct p, p, p, p.
+    specialize (sLd a p d1 d).
+    specialize (sSt a p d1 d).
+    specialize (bLd a p d1 (if d0 then getNStateForStm stm getTransIo 0 a else initData zero)).
+    specialize (bSt a p d1 (if d0 then getNStateForStm stm getTransIo 0 a else initData zero)).
+
+    case_eq (getStreamIo getImIo 0 (buildIm stm getTransIo 0)); intros.
+    simpl in H, sth.
+    rewrite H in *; clear H.
+    destruct p0, p0, p0, p0.
+    destruct sth as [u1 [u2 [u3 [u4 u5]]]].
+    rewrite u1, u2, u3, u4, u5 in *; clear u1 u2 u3 u4.
+    repeat f_equal.
+
+    destruct d3.
+
+    assert (Some (a0, p0, d4, Ld, d) = Some (a0, p0, d4, Ld, d)) by reflexivity.
+    specialize (sLd H); clear H.
+    assert (Some (a0, p0, d4, Ld, getNStateForStm stm getTransIo 0 a0) =
+            Some (a0, p0, d4, Ld, getNStateForStm stm getTransIo 0 a0)) by reflexivity.
+    specialize (bLd H); clear H.
+
+    destruct sLd, bLd.
+    intuition.
+    intuition.
+    destruct H as [_ [tb [_ [x _]]]].
+    assert False by omega; intuition.
+    destruct H as [_ [tb [_ [x _]]]].
+    assert False by omega; intuition.
+
+    assert (Some (a0, p0, d4, St, d) = Some (a0, p0, d4, St,d)) by reflexivity.
+    apply (sSt H).
+
+
+    simpl in H, sth.
+    rewrite H in *; clear H.
+    intuition.
+
+    case_eq (getStreamIo getImIo 0 (buildIm stm getTransIo 0)); intros.
+    simpl in H, sth.
+    rewrite H in *; clear H.
+    intuition.
+    auto.
+
+
+
+    intros n IHn.
+
+
+
+
+    simpl in *.
+    destruct sa as [sLd sSt].
+
+    pose proof (saInstMem (buildIm stm getTransIo 0)) as [bLd bSt].
+    specialize (sLd (S n)).
+    specialize (sSt (S n)).
+    specialize (bLd (S n)).
+    specialize (bSt (S n)).
+
+    pose proof (buildImSth stm getTransIo (S n) 0) as sth; assert (H:S n+0 = S n) by omega;
+    rewrite H in *; clear H.
+
+
+    destruct (getStreamIo getTransIo (S n) stm).
+    destruct p, p, p, p.
+    specialize (sLd a p d1 d).
+    specialize (sSt a p d1 d).
+    specialize (bLd a p d1 (if d0 then getNStateForStm stm getTransIo (S n) a else initData zero)).
+    specialize (bSt a p d1 (if d0 then getNStateForStm stm getTransIo (S n) a else initData zero)).
+
+    case_eq (getStreamIo getImIo (S n) (buildIm stm getTransIo 0)); intros.
+    simpl in H.
+    unfold getNStateForStm at 1 in sth.
+    rewrite H in *; clear H.
+    destruct p0, p0, p0, p0.
+    destruct sth as [u1 [u2 [u3 [u4 u5]]]].
+    rewrite u1, u2, u3, u4, u5 in *.
+    clear u1 u2 u3 u4.
+    repeat f_equal.
+
+    destruct d3.
+
+    assert (Some (a0, p0, d4, Ld, d) = Some (a0, p0, d4, Ld, d)) by reflexivity.
+    specialize (sLd H); clear H.
+    assert (Some (a0, p0, d4, Ld, getNStateForStm stm getTransIo (S n) a0) =
+            Some (a0, p0, d4, Ld, getNStateForStm stm getTransIo (S n) a0)) by reflexivity.
+    specialize (bLd H); clear H.
+
+    destruct sLd, bLd.
+    destruct H as [u1 _]; destruct H0 as [u2 _].
+    rewrite <- u2 in u1.
+    assumption.
+
+    destruct H as [_ u1]; destruct H0 as [cb [tb [ldb [lt [eq _]]]]].
+    assert (0 <= tb < S n) by omega.
+    rewrite <- u5 in eq.
+    assert (H0: tb <= n) by omega.
+    specialize (IHn tb H0).
+    rewrite <- IHn in eq.
+    specialize (u1 tb H cb d2 ldb eq); intuition.
+
+    destruct H0 as [_ u1]; destruct H as [cb [tb [ldb [lt [eq _]]]]].
+    assert (0 <= tb < S n) by omega.
+    assert (H0: tb <= n) by omega.
+    specialize (IHn tb H0).
+    rewrite IHn in eq.
+    specialize (u1 tb H cb d ldb eq); intuition.
+
+
+
+
+
+
+    destruct H as [cb [tb [ldb [lt [eq rest] ]]]];
+      destruct H0 as [cb' [tb' [ldb' [lt' [eq' rest']]]]].
+
+
+    assert (opts:tb = tb' \/ tb < tb' \/ tb > tb') by omega.
+
+    destruct opts as [ez | [hard1  | hard2]].
+
+    rewrite ez in *.
+
+    assert (H: tb' <= n) by omega.
+    specialize (IHn tb' H).
+    rewrite IHn in *.
+    rewrite eq in eq'.
+    injection eq'; intros; assumption.
+
+
+    specialize (rest tb' (conj hard1 lt') cb' (getNStateForStm stm getTransIo (S n) a0) ldb').
+    assert (H: tb' <= n) by omega.
+    specialize (IHn tb' H).
+    rewrite IHn in *.
+    intuition.
+
+
+    specialize (rest' tb (conj hard2 lt) cb d ldb).
+    assert (H: tb <= n) by omega.
+    specialize (IHn tb H).
+    rewrite IHn in *.
+    intuition.
+
+    assert (Some (a0, p0, d4, St, d) = Some (a0, p0, d4, St, d)) by reflexivity.
+    intuition.
+
+
+    rewrite H in *.
+    intuition.
+
+
+    case_eq (getStreamIo getImIo (S n) (buildIm stm getTransIo 0)); intros.
+    simpl in H.
+    unfold getNStateForStm at 1 in sth.
+    rewrite H in *; clear H.
+    intuition.
+
+    auto.
+  Qed.
+End Final.
